mipstlb: clean up proofs
Signed-off-by: Reto Achermann <reto.achermann@inf.ethz.ch>

theories/mipstlb/MipsTLBEquivalence.thy
@@ -36,9 +36,9 @@ begin
 section "Equivalence to Large TLB"
 (* ========================================================================= *)  
 
-text "Next we show that for all " 
+text "Next we show that for all valid TLBs the TLB with replacement handler
+      behaves as if its  " 
 
-    
   
 lemma TLBEquivalence :
     assumes inrange: "vpn < MIPSPT_EntriesMax"
@@ -63,6 +63,14 @@ proof -
   from X0 X1 show ?thesis by(auto)
 qed
 
+
+(* ========================================================================= *)  
+section "Equivalence in decoding net nodes"
+(* ========================================================================= *) 
+
+text "First we define a few helper functions that convert virtual addresses
+     into (asid, vpn, offset)"
+
 definition addr2vpn :: "addr \<Rightarrow> VPN"
   where "addr2vpn a = ((fst a) mod VASize) div 4096"
 
@@ -72,9 +80,16 @@ definition addr2asid :: "addr \<Rightarrow> ASID"
 definition pfn2addr :: "PFN \<Rightarrow> addr \<Rightarrow> addr"
   where "pfn2addr p va = (p * 4096 + (fst va) mod 4096, {})"
 
+
+text "A virtual address is valid, if it's representable by the available bits
+      i.e.. 8-bit ASID and 40-bit Address"
+
 definition AddrValid :: "addr \<Rightarrow> bool"
   where "AddrValid a = ((fst a) < VASize * ASIDMax)"
 
+
+text "If the address is valid, then extracting the ASID and VPN is within the well
+      defined ranges."
 
 lemma AddrValid_implies_inrange :
   "AddrValid a \<Longrightarrow> addr2vpn a < MIPSPT_EntriesMax"
@@ -84,26 +99,46 @@ lemma AddrValid_implies_inrange2 :
   "AddrValid a \<Longrightarrow> addr2asid a < ASIDMax"
   by(auto simp:addr2asid_def AddrValid_def VASize_def ASIDMax_def MIPSPT_EntriesMax_def)
 
+(* ------------------------------------------------------------------------- *)  
+subsection "Lifting methods"
+(* ------------------------------------------------------------------------- *) 
+
+text "We construct decoding net nodes for both, the large TLB and the 
+      replacement handler by using their translate functions"
 
 definition MipsTLBPT_to_node :: "nodeid \<Rightarrow> MipsTLBPT \<Rightarrow> node"
-  where "MipsTLBPT_to_node nid mpt =  \<lparr> accept = {},
-         translate = (\<lambda>a. (if AddrValid a then 
-         (\<Union>x\<in> (MipsTLBPT_translate mpt (addr2asid a) (addr2vpn a)). {(nid, pfn2addr x a)} )  else {} ))  \<rparr>"
+  where "MipsTLBPT_to_node nid mpt =  \<lparr> 
+          accept = {},
+          translate = (\<lambda>a. 
+            (if AddrValid a then 
+              (\<Union>x\<in> (MipsTLBPT_translate mpt (addr2asid a) (addr2vpn a)). {(nid, pfn2addr x a)} )  
+            else {} ))  \<rparr>"
 
 
 definition MIPSLARGE_to_node :: "nodeid \<Rightarrow> MIPSTLB \<Rightarrow> node"
-  where "MIPSLARGE_to_node nid t =  \<lparr> accept = {},
-        translate = (\<lambda>a.  (if AddrValid a then 
-        (\<Union>x\<in> (MIPSTLB_translate t (addr2asid a) (addr2vpn a)). {(nid, pfn2addr x a)} ) else {} ))  \<rparr>"
+  where "MIPSLARGE_to_node nid t =  \<lparr> 
+          accept = {},
+          translate = (\<lambda>a.  
+            (if AddrValid a then 
+              (\<Union>x\<in> (MIPSTLB_translate t (addr2asid a) (addr2vpn a)). {(nid, pfn2addr x a)} ) 
+             else {} ))  \<rparr>"
 
 
+(* ------------------------------------------------------------------------- *)  
+subsection "Equivalence Proof of lifted nodes"
+(* ------------------------------------------------------------------------- *) 
 
-lemma Equiv :
+text "We first define a lemma that shows that if the address is valid, then the
+      set of translated addresses  are the same. "
+
+lemma translate_function_equivalent :
   assumes cap: "capacity (tlb mpt) > 0"
       and valid: "MipsTLBPT_valid mpt"
       and avalid: "AddrValid a"
-    shows "(\<Union>x\<in>MipsTLBPT_translate mpt (addr2asid a) (addr2vpn a). {(nid, pfn2addr x a)})  = 
-           ( \<Union>x\<in>MIPSTLB_translate (MipsTLBLarge_create (pte mpt)) (addr2asid a) (addr2vpn a). {(nid, pfn2addr x a)})"
+    shows "(\<Union>x\<in>MipsTLBPT_translate mpt (addr2asid a) (addr2vpn a). 
+                {(nid, pfn2addr x a)})  = 
+           (\<Union>x\<in>MIPSTLB_translate (MipsTLBLarge_create (pte mpt)) (addr2asid a) (addr2vpn a). 
+                {(nid, pfn2addr x a)})"
 proof -
   from avalid have X0: "addr2asid a < ASIDMax"
     by(auto simp:AddrValid_implies_inrange2)
@@ -115,6 +150,7 @@ proof -
     by(auto simp: TLBEquivalence)
 qed
 
+text "Next, we use the lemma above to proof that the two nodes will be the same."
 
 lemma 
   assumes cap: "capacity (tlb mpt) > 0"
@@ -122,25 +158,45 @@ lemma
   shows "MipsTLBPT_to_node nid mpt = 
          MIPSLARGE_to_node nid (MipsTLBLarge_create (pte mpt))"
 proof -
-  have X0:  "MipsTLBPT_to_node nid mpt =  \<lparr>accept = {}, translate = \<lambda>a. if AddrValid a then \<Union>x\<in>MipsTLBPT_translate mpt (addr2asid a) (addr2vpn a). {(nid, pfn2addr x a)} else {}\<rparr>"
+  have X0:  
+    "MipsTLBPT_to_node nid mpt =  \<lparr>
+      accept = {}, 
+      translate = \<lambda>a. if AddrValid a 
+        then \<Union>x\<in>MipsTLBPT_translate mpt (addr2asid a) (addr2vpn a). {(nid, pfn2addr x a)} 
+        else {}\<rparr>"
     by(simp add:MipsTLBPT_to_node_def)
 
-  have X1: " MIPSLARGE_to_node nid (MipsTLBLarge_create (pte mpt)) =  \<lparr>accept = {}, translate = \<lambda>a. if AddrValid a then \<Union>x\<in>MIPSTLB_translate (MipsTLBLarge_create (pte mpt)) (addr2asid a) (addr2vpn a). {(nid, pfn2addr x a)} else {}\<rparr>"
+  have X1: 
+    "MIPSLARGE_to_node nid (MipsTLBLarge_create (pte mpt)) =  \<lparr>
+      accept = {}, 
+      translate = \<lambda>a. if AddrValid a 
+        then \<Union>x\<in>MIPSTLB_translate (MipsTLBLarge_create (pte mpt)) 
+                       (addr2asid a) (addr2vpn a). {(nid, pfn2addr x a)}
+        else {}\<rparr>"
     by(simp add:MIPSLARGE_to_node_def)
 
-  from cap valid have X2: "\<And>a. (if AddrValid a then \<Union>x\<in>MipsTLBPT_translate mpt (addr2asid a) (addr2vpn a). {(nid, pfn2addr x a)} else {}) = 
-             (if AddrValid a then \<Union>x\<in>MIPSTLB_translate (MipsTLBLarge_create (pte mpt)) (addr2asid a) (addr2vpn a). {(nid, pfn2addr x a)} else {})"
-    by(auto simp:Equiv)
+  from cap valid have X2: 
+    "\<And>a. (if AddrValid a then \<Union>x\<in>MipsTLBPT_translate mpt (addr2asid a) (addr2vpn a).
+             {(nid, pfn2addr x a)} else {}) = 
+          (if AddrValid a then \<Union>x\<in>MIPSTLB_translate (MipsTLBLarge_create (pte mpt)) 
+             (addr2asid a) (addr2vpn a). {(nid, pfn2addr x a)} else {})"
+    by(auto simp:translate_function_equivalent)
 
-
-  from X0 cap valid have X3 :  " \<lparr>accept = {}, translate = \<lambda>a. if AddrValid a then \<Union>x\<in>MipsTLBPT_translate mpt (addr2asid a) (addr2vpn a). {(nid, pfn2addr x a)} else {}\<rparr> = 
-                  \<lparr>accept = {}, translate = \<lambda>a. if AddrValid a then \<Union>x\<in>MIPSTLB_translate (MipsTLBLarge_create (pte mpt)) (addr2asid a) (addr2vpn a). {(nid, pfn2addr x a)} else {}\<rparr>"
+  from X0 cap valid have X3: 
+    "\<lparr>accept = {}, 
+     translate = \<lambda>a. 
+        if AddrValid a 
+          then \<Union>x\<in>MipsTLBPT_translate mpt (addr2asid a) (addr2vpn a). {(nid, pfn2addr x a)} 
+        else {} \<rparr> = 
+      \<lparr>accept = {}, 
+       translate = \<lambda>a. 
+        if AddrValid a 
+          then \<Union>x\<in>MIPSTLB_translate (MipsTLBLarge_create (pte mpt)) 
+                          (addr2asid a) (addr2vpn a). {(nid, pfn2addr x a)} 
+        else {}\<rparr>"
     by(simp only:X2)
 
   from X0 X1 X2 show ?thesis by(auto)
 qed
-
-
-
 
 end  
